Wasm_Inference_Rules.thy
@@ -1,38 +1,23 @@
 theory Wasm_Inference_Rules imports Wasm_Assertions_Shallow begin
 
-definition stack_ass_ind_on_glob :: "'a stack_ass \<Rightarrow> nat \<Rightarrow> bool" where
-  "stack_ass_ind_on_glob St n \<equiv>
-     (\<forall>vs v_st g. stack_ass_sat St vs v_st = (stack_ass_sat St vs (var_st_set_global v_st n g)))"
+definition var_st_differ_on :: "'a var_st \<Rightarrow> var set \<Rightarrow> 'a var_st \<Rightarrow> bool" where
+  "var_st_differ_on v_st vars v_st' \<equiv> (\<forall>var. var \<notin> vars \<longrightarrow> var_st_agree v_st var v_st')"
 
-definition stack_ass_ind_on_loc :: "'a stack_ass \<Rightarrow> nat \<Rightarrow> bool" where
-  "stack_ass_ind_on_loc St n \<equiv>
-     (\<forall>vs v_st l. stack_ass_sat St vs v_st = (stack_ass_sat St vs (var_st_set_local v_st n l)))"
+lemma var_st_differ_on_refl: "var_st_differ_on v_st vars v_st"
+  unfolding var_st_differ_on_def var_st_agree_def
+  by (auto split: var.splits)
 
-definition stack_ass_ind_on :: "'a stack_ass \<Rightarrow> var \<Rightarrow> bool" where
-  "stack_ass_ind_on H var \<equiv> case var of
-                             Gl n \<Rightarrow> stack_ass_ind_on_glob H n
-                           | Lc n \<Rightarrow> stack_ass_ind_on_loc H n
-                           | Lv n \<Rightarrow> True"
+definition stack_ass_ind_on :: "'a stack_ass \<Rightarrow> var set \<Rightarrow> bool" where
+  "stack_ass_ind_on St vars \<equiv> \<forall>vs v_st v_st'. var_st_differ_on v_st vars v_st' \<longrightarrow> stack_ass_sat St vs v_st = stack_ass_sat St vs v_st'"
 
-definition heap_ass_ind_on_glob :: "'a heap_ass \<Rightarrow> nat \<Rightarrow> bool" where
-  "heap_ass_ind_on_glob H n \<equiv>
-     (\<forall>h v_st g. H h v_st = (H h (var_st_set_global v_st n g)))"
-
-definition heap_ass_ind_on_loc :: "'a heap_ass \<Rightarrow> nat \<Rightarrow> bool" where
-  "heap_ass_ind_on_loc H n \<equiv>
-     (\<forall>h v_st l. H h v_st = (H h (var_st_set_local v_st n l)))"
-
-definition heap_ass_ind_on :: "'a heap_ass \<Rightarrow> var \<Rightarrow> bool" where
-  "heap_ass_ind_on H var \<equiv> case var of
-                             Gl n \<Rightarrow> heap_ass_ind_on_glob H n
-                           | Lc n \<Rightarrow> heap_ass_ind_on_loc H n
-                           | Lv n \<Rightarrow> True"
+definition heap_ass_ind_on :: "'a heap_ass \<Rightarrow> var set \<Rightarrow> bool" where
+  "heap_ass_ind_on H vars \<equiv> \<forall>h v_st v_st'. var_st_differ_on v_st vars v_st' \<longrightarrow> H h v_st = H h v_st'"
 
 context encapsulated_module
 begin
 
 inductive modifies :: "cl list \<Rightarrow> e list \<Rightarrow> var \<Rightarrow> bool" where
-"\<lbrakk>(modifies fs es v) \<or> (modifies fs es' v)\<rbrakk> \<Longrightarrow> modifies fs (es@es') v"
+"\<lbrakk>(modifies fs [e] v) \<or> (modifies fs es v)\<rbrakk> \<Longrightarrow> modifies fs (e#es) v"
 | "modifies fs [$Set_local j] (Lc j)"
 | "modifies fs [$Tee_local j] (Lc j)"
 | "modifies fs [$Set_global j] (Gl j)"
@@ -44,149 +29,265 @@ inductive modifies :: "cl list \<Rightarrow> e list \<Rightarrow> var \<Rightarr
 | "\<lbrakk>(modifies fs es v)\<rbrakk> \<Longrightarrow> modifies fs [Local _ i lvs es] v"
 | "\<lbrakk>cl = Func_native i _ _ b_es; (modifies fs ($* b_es) v)\<rbrakk> \<Longrightarrow> modifies fs [Callcl cl] v"
 
-lemma refl_var_st:
-  assumes "reifies_glob (globs s) (inst.globs i) var_st"
-          "reifies_loc vs var_st"
-          "snd (snd var_st) = lvar_st"
-          "reifies_glob (globs s) (inst.globs i) var_st'"
-          "reifies_loc vs var_st'"
-          "snd (snd var_st') = lvar_st"
-  shows "var_st_agree var_st v var_st'"
-proof (cases v)
-  case (Gl x1)
-  thus ?thesis
-    using assms(1,4)
-    unfolding var_st_agree_def var_st_get_global_def reifies_glob_def
-    apply (cases var_st; cases var_st')
-    apply auto
-    done
-next
-  case (Lc x2)
-  thus ?thesis
-    using assms(2,5)
-    unfolding var_st_agree_def var_st_get_local_def reifies_loc_def
+
+definition modset where "modset cls es = {v. modifies cls es v}"
+
+lemma modifies_modset_eq [pred_set_conv]: "modifies cl es = (\<lambda>v. v \<in> modset cl es)"
+by(simp add: modset_def)
+
+lemmas modset_intros [intro?] = modifies.intros[to_set]
+lemmas modset_induct [consumes 1, induct set: modset] = modifies.induct[to_set]
+lemmas modset_cases [consumes 1, cases set: modset] = modifies.cases[to_set]
+lemmas modset_simps = modifies.simps[to_set]
+
+lemma modset_consts:
+  assumes "x \<in> modset fs ($$*vs)"
+  shows "False"
+  using assms
+proof (induction fs "($$*vs)" x arbitrary: vs rule: modset_induct)
+  case (1 fs e v es)
+  thus ?case
+    using consts_app_ex[of "[e]" "es"]
+    by (metis append_Nil append_eq_Cons_conv)
+qed auto
+
+lemma modset_emp:
+  assumes "x \<in> modset fs []"
+  shows "False"
+  using assms modset_consts[of x fs "[]"]
+  by auto
+
+lemma modset_cons:
+  assumes "m \<in> modset fs es"
+          "es = e1#es2"
+  shows "m \<in> modset fs [e1] \<or> m \<in> modset fs es2"
+  using assms
+  by (induction rule: modset_induct) (auto intro: modset_intros)
+
+lemma modset_arb_app1:
+  assumes "m \<in> modset fs es"
+          "es = es1@es2"
+  shows "m \<in> modset fs es1 \<or> m \<in> modset fs es2"
+  using assms
+proof (induction es1 arbitrary: es es2)
+  case Nil
+  thus ?case
     by simp
 next
-  case (Lv x3)
-  thus ?thesis
-    using assms(3,6)
-    unfolding var_st_agree_def var_st_get_lvar_def
-    by simp
+  case (Cons e es1)
+  hence "m \<in> modset fs [e] \<or> m \<in> modset fs (es1@es2)"
+    using modset_cons
+    by fastforce
+  thus ?case
+    using Cons modset_intros(1) 
+    by blast
 qed
+
+lemma modset_arb_app:
+  assumes "m \<in> modset fs es1 \<or> m \<in> modset fs es2"
+  shows "m \<in> modset fs (es1@es2)"
+  using assms
+proof (induction es1)
+  case Nil
+  thus ?case
+    using modset_emp
+    by fastforce
+next
+  case (Cons a es1)
+  thus ?case
+    by (metis append_Cons modset_intros(1) modset_cons)
+qed
+
+lemma modset_consts_app:
+  "(m \<in> modset fs (($$*vs)@es)) = (m \<in> modset fs es)"
+  using modset_arb_app modset_arb_app1 modset_consts
+  by blast
 
 lemma modifies_var_st:
   assumes "(s,vs,es) \<Down>k{(ls,r,i)} (s',vs',res)"
           "reifies_func (funcs s) (inst.funcs i) fs"
           "reifies_glob (globs s) (inst.globs i) var_st"
-          "snd (snd var_st) = lvar_st"
           "reifies_loc vs var_st"
-          "\<not>(modifies fs es v)"
+          "snd (snd var_st) = lvar_st"
           "reifies_glob (globs s') (inst.globs i) var_st'"
           "reifies_loc vs' var_st'"
           "snd (snd var_st') = lvar_st"
-  shows "var_st_agree var_st v var_st'"
+  shows "var_st_differ_on var_st (modset fs es) var_st'"
   using assms
 proof (induction "(s,vs,es)" k "(ls,r,i)" "(s',vs',res)" arbitrary: s vs es s' vs' res rule: reduce_to_n.induct)
-  case (block ves n t1s t2s m es k)
-  thus ?case sorry
+case (const s vs v k)
+then show ?case sorry
 next
-  case (loop ves n t1s t2s m es k)
+  case (unop s vs v t op k)
   then show ?case sorry
 next
-  case (if_false n ves tf e2s k e1s)
+  case (binop_Some op v1 v2 v s vs t k)
   then show ?case sorry
 next
-  case (if_true n ves tf e1s k e2s)
+case (binop_None op v1 v2 s vs t k)
   then show ?case sorry
 next
-  case (br_if_true n ves j k)
+case (testop s vs v t op k)
   then show ?case sorry
 next
-  case (br_table js c ves k j)
+case (relop s vs v1 v2 t op k)
   then show ?case sorry
 next
-  case (br_table_length js c ves j k)
+case (convert_Some t1 v t2 sx v' s vs k)
   then show ?case sorry
 next
-  case (return r vcs k)
+case (convert_None t1 v t2 sx s vs k)
   then show ?case sorry
 next
-  case (set_local vi j v vs v' k)
+  case (reinterpret t1 v s vs t2 k)
+then show ?case sorry
+next
+  case (unreachable s vs k)
   then show ?case sorry
 next
-  case (tee_local v i k)
+case (nop s vs k)
   then show ?case sorry
 next
-  case (set_global j v k)
+  case (drop s vs v k)
   then show ?case sorry
 next
-  case (store_Some t v j m n off mem' a k)
+  case (select_false n s vs v1 v2 k)
   then show ?case sorry
 next
-  case (store_packed_Some t v j m n off tp mem' a k)
+  case (select_true n s vs v1 v2 k)
   then show ?case sorry
 next
-  case (grow_memory j m n c mem' k)
+  case (block ves n t1s t2s m s vs es k s' vs' res)
   then show ?case sorry
 next
-  case (call ves j k)
+case (loop ves n t1s t2s m s vs es k s' vs' res)
   then show ?case sorry
 next
-  case (call_indirect_Some c cl j tf ves k)
+  case (if_false n ves s vs tf e2s k s' vs' res e1s)
   then show ?case sorry
 next
-  case (callcl_native cl j t1s t2s ts es ves vcs n m zs k)
+  case (if_true n ves s vs tf e1s k s' vs' res e2s)
   then show ?case sorry
 next
-  case (callcl_host_Some cl t1s t2s f ves vcs n m hs vcs' k)
+  case (br vcs n j s vs k)
   then show ?case sorry
 next
-  case (callcl_host_None cl t1s t2s f ves vcs n m k)
+  case (br_if_false n s vs j k)
   then show ?case sorry
 next
-  case (const_value es k res ves)
+  case (br_if_true n ves s vs j k s' vs' res)
   then show ?case sorry
 next
-  case (label_value es k n res les)
+  case (br_table js c ves s vs k s' vs' res j)
   then show ?case sorry
 next
-  case (local_value lls es k n j lls' res)
+  case (br_table_length js c ves s vs j k s' vs' res)
   then show ?case sorry
 next
-  case (seq_value es k s'' vs'' res'' es' res)
+  case (return vs r s vcs k)
+then show ?case sorry
+next
+  case (get_local vi j s v vs k)
   then show ?case sorry
 next
-  case (seq_nonvalue ves es k es')
+  case (set_local vi j s v vs v' k)
   then show ?case sorry
 next
-  case (label_trap es k n les)
+  case (tee_local v s vs i k s' vs' res)
   then show ?case sorry
 next
-  case (local_trap lls es k n j lls')
+  case (get_global s vs j k)
   then show ?case sorry
 next
-  case (label_break_suc es k n bn bvs les)
+  case (set_global s j v s' vs k)
   then show ?case sorry
 next
-  case (label_break_nil es k n s'' vs'' bvs es' \<Gamma> les)
+  case (load_Some s j m n off t bs vs a k)
   then show ?case sorry
 next
-  case (label_return es k n rvs les)
-  thus ?case sorry
+  case (load_None s j m n off t vs a k)
+  then show ?case sorry
 next
-  case (local_return lls es k n j lls' rvs)
-  thus ?case sorry
-qed (metis refl_var_st)+
-
-lemma Hf_equiv:
-  assumes "\<And>v. var_st_agree var_st v var_st' \<or> heap_ass_ind_on Hf v"
-          "snd (snd var_st) = lvar_st"
-          "snd (snd var_st') = lvar_st"
-  shows "Hf h var_st = Hf h var_st'"
-proof -
-  show ?thesis
-    sorry
+  case (load_packed_Some s j m sx n off tp t bs vs a k)
+  then show ?case sorry
+next
+  case (load_packed_None s j m sx n off tp t vs a k)
+then show ?case sorry
+next
+  case (store_Some t v s j m n off mem' vs a k)
+  then show ?case sorry
+next
+  case (store_None t v s j m n off vs a k)
+  then show ?case sorry
+next
+  case (store_packed_Some t v s j m n off tp mem' vs a k)
+then show ?case sorry
+next
+  case (store_packed_None t v s j m n off tp vs a k)
+  then show ?case sorry
+next
+  case (current_memory s j m n vs k)
+  then show ?case sorry
+next
+  case (grow_memory s j m n c mem' vs k)
+  then show ?case sorry
+next
+  case (grow_memory_fail s j m n vs c k)
+  then show ?case sorry
+next
+  case (call ves s vs j k s' vs' res)
+  then show ?case sorry
+next
+  case (call_indirect_Some s c cl j tf ves vs k s' vs' res)
+  then show ?case sorry
+next
+  case (call_indirect_None s c cl j vs k)
+  then show ?case sorry
+next
+  case (callcl_native cl j t1s t2s ts es ves vcs n m zs s vs k s' vs' res)
+  then show ?case sorry
+next
+  case (callcl_host_Some cl t1s t2s f ves vcs n m s hs s' vcs' vs k)
+  then show ?case sorry
+next
+  case (callcl_host_None cl t1s t2s f ves vcs n m s vs k)
+  then show ?case sorry
+next
+  case (const_value s vs es k s' vs' res ves)
+  then show ?case sorry
+next
+  case (label_value s vs es k n s' vs' res les)
+  then show ?case sorry
+next
+  case (local_value s lls es k n j s' lls' res vs)
+  then show ?case sorry
+next
+  case (seq_value s vs es k s'' vs'' res'' es' s' vs' res)
+then show ?case sorry
+next
+  case (seq_nonvalue ves s vs es k s' vs' res es')
+  then show ?case sorry
+next
+  case (label_trap s vs es k n s' vs' les)
+  then show ?case sorry
+next
+  case (local_trap s lls es k n j s' lls' vs)
+  then show ?case sorry
+next
+  case (label_break_suc s vs es k n s' vs' bn bvs les)
+  then show ?case sorry
+next
+  case (label_break_nil s vs es k n s'' vs'' bvs es' \<Gamma> s' vs' res les)
+  then show ?case sorry
+next
+  case (label_return s vs es k n s' vs' rvs les)
+  then show ?case sorry
+next
+  case (local_return s lls es k n j s' lls' rvs vs)
+  then show ?case sorry
 qed
+
+
 
 definition pred_option_Some :: "('a \<Rightarrow> bool) \<Rightarrow> 'a option \<Rightarrow> bool" where
   "pred_option_Some pred opt \<equiv> opt \<noteq> None \<and> pred_option pred opt"
@@ -194,6 +295,25 @@ definition pred_option_Some :: "('a \<Rightarrow> bool) \<Rightarrow> 'a option 
 (* separating conjuction *)
 definition sep_conj :: "'a heap_ass \<Rightarrow> 'a heap_ass \<Rightarrow> 'a heap_ass" (infixr "\<^emph>" 60) where
   "ha' \<^emph> ha'' \<equiv> \<lambda>h st. \<exists>h' h''. heap_disj h' h'' \<and> ha' h' st \<and> ha'' h'' st \<and> heap_merge h' h'' = h"
+
+definition ass_frame :: "'a heap_ass \<Rightarrow> 'a ass \<Rightarrow> 'a ass" where
+  "ass_frame F ass \<equiv> (case ass of
+                        (St \<^sub>s|\<^sub>h H) \<Rightarrow>  St \<^sub>s|\<^sub>h (H \<^emph> F)
+                      | x \<Rightarrow> x)"
+
+lemma ass_stack_len_ass_frame_inv: "ass_stack_len (ass_frame Hf ass) = ass_stack_len ass"
+  unfolding ass_frame_def
+  apply (cases ass)
+   apply auto
+  done
+
+lemma reifies_lab_ass_frame_inv: "reifies_lab labs (fs, map (ass_frame Hf) ls,  rs) = reifies_lab labs (fs, ls, rs)"
+  unfolding reifies_lab_def
+  by (auto simp add: ass_stack_len_ass_frame_inv)
+
+lemma reifies_ret_ass_frame_inv: "reifies_ret ret (fs, ls, map_option (ass_frame Hf) rs) = reifies_ret ret (fs, ls, rs)"
+  unfolding reifies_ret_def
+  by (metis (no_types, lifting) ass_stack_len_ass_frame_inv not_Some_eq option.simps(8,9) prod.sel(2))
 
 definition args_ass :: "'a stack_ass \<Rightarrow> nat \<Rightarrow> 'a var_st \<Rightarrow> bool" where
   "args_ass St n v_st \<equiv> (length St = n \<and> (\<forall>i < n. pred_option_Some (\<lambda>v. (St!i) v v_st) (var_st_get_local v_st i)))"
@@ -225,8 +345,8 @@ inductive inf_triples :: "'a triple_context \<Rightarrow> 'a triple set \<Righta
 | Asm:"\<lbrakk>(P, [$Call k], Q) \<in> assms\<rbrakk> \<Longrightarrow> \<Gamma>\<bullet>assms \<turnstile> {P} [$Call k] {Q}"
 | Seq:"\<lbrakk>\<Gamma>\<bullet>assms \<turnstile> {P} es {Q}; \<Gamma>\<bullet>assms \<turnstile> {Q} es' {R}\<rbrakk> \<Longrightarrow> \<Gamma>\<bullet>assms \<turnstile> {P} es@es' {R}"
 | Conseq:"\<lbrakk>\<Gamma>\<bullet>assms \<turnstile> {P'} es {Q'}; \<forall>vs h vs_t. (ass_sat P vs h vs_t \<longrightarrow> ass_sat P' vs h vs_t) \<and> (ass_sat Q' vs h vs_t \<longrightarrow> ass_sat Q vs h vs_t)\<rbrakk> \<Longrightarrow> \<Gamma>\<bullet>assms \<turnstile> {P} es {Q}"
-| Frame:"\<lbrakk>\<Gamma>\<bullet>assms \<turnstile> {St \<^sub>s|\<^sub>h H} es {St' \<^sub>s|\<^sub>h H'}; (\<forall>v. modifies fs es v \<longrightarrow> heap_ass_ind_on Hf v)\<rbrakk> \<Longrightarrow> \<Gamma>\<bullet>assms \<turnstile> {St \<^sub>s|\<^sub>h (H \<^emph> Hf)} es {St' \<^sub>s|\<^sub>h (H' \<^emph> Hf)}"
-| Ext:"\<lbrakk>\<Gamma>\<bullet>assms \<turnstile> {St \<^sub>s|\<^sub>h H} es {St' \<^sub>s|\<^sub>h H'}; (\<forall>v. modifies fs es v \<longrightarrow> stack_ass_ind_on Stf v)\<rbrakk> \<Longrightarrow> \<Gamma>\<bullet>assms \<turnstile> {(Stf @ St) \<^sub>s|\<^sub>h H} es {(Stf @ St') \<^sub>s|\<^sub>h H'}"
+| Frame:"\<lbrakk>(fs,ls,rs)\<bullet>assms \<turnstile> {St \<^sub>s|\<^sub>h H} es {St' \<^sub>s|\<^sub>h H'}; heap_ass_ind_on Hf (modset fs es); (\<forall>ass \<in> (set ls). \<exists>Sa Ha. ass = Sa \<^sub>s|\<^sub>h Ha); pred_option (\<lambda>ass. \<exists>Sa Ha. ass = Sa \<^sub>s|\<^sub>h Ha) rs\<rbrakk> \<Longrightarrow> (fs,map (ass_frame Hf) ls, map_option (ass_frame Hf) rs)\<bullet>assms \<turnstile> {St \<^sub>s|\<^sub>h (H \<^emph> Hf)} es {St' \<^sub>s|\<^sub>h (H' \<^emph> Hf)}"
+| Ext:"\<lbrakk>\<Gamma>\<bullet>assms \<turnstile> {St \<^sub>s|\<^sub>h H} es {St' \<^sub>s|\<^sub>h H'}; stack_ass_ind_on Stf (modset (fst \<Gamma>) es)\<rbrakk> \<Longrightarrow> \<Gamma>\<bullet>assms \<turnstile> {(Stf @ St) \<^sub>s|\<^sub>h H} es {(Stf @ St') \<^sub>s|\<^sub>h H'}"
 | Call:"\<lbrakk>(fs,[],None)\<bullet>specs \<tturnstile> ({(P,c,Q). \<exists>i. (P, [$Call i], Q) \<in> specs \<and> i< length fs \<and> c = [Callcl (fs!i)]}); \<forall>(P,c,Q) \<in> specs. \<exists>i. c = [$Call i] \<and> i < length fs\<rbrakk> \<Longrightarrow> (fs,[],None)\<bullet>({}) \<tturnstile> specs"
 | ConjI:"\<forall>(P,es,Q) \<in> specs. (\<Gamma>\<bullet>assms \<turnstile> {P} es {Q}) \<Longrightarrow> \<Gamma>\<bullet>assms \<tturnstile> specs"
 | ConjE:"\<lbrakk>\<Gamma>\<bullet>assms \<tturnstile> specs; (P,es,Q) \<in> specs\<rbrakk> \<Longrightarrow> \<Gamma>\<bullet>assms \<turnstile> {P} es {Q}"
@@ -254,6 +374,322 @@ proof -
   thus ?thesis
     unfolding valid_triple_n_def
     by metis
+qed
+
+lemma sep_conj_imp_frame:
+  assumes   "stack_ass_sat St vcs st"
+            "heap_disj h_H h_Hf"
+            "H h_H st"
+            "Hf h_Hf st"
+            "heap_merge h_H h_Hf = h"
+            "heap_disj h hf"
+            "reifies_s s i (heap_merge h hf) st (fst \<Gamma>)"
+            "reifies_loc locs st"
+            "reifies_lab labs \<Gamma>"
+            "reifies_ret ret \<Gamma>"
+            "snd (snd st) = lvar_st"
+  shows "(ass_wf lvar_st ret \<Gamma> labs locs s (heap_merge h_Hf hf) st h_H vcs (St \<^sub>s|\<^sub>h H))"
+proof -
+  show ?thesis
+    using assms
+    unfolding ass_wf_def
+    by (auto simp add: heap_merge_assoc heap_disj_merge_assoc)
+qed
+
+lemma res_wf_intro_value:
+  assumes "ass_sat (St' \<^sub>s|\<^sub>h H') vcs' h'' st'"
+          "rvs = vcsf @ vcs'"
+          "heap_disj h'' hf"
+          "h' = heap_merge h'' hf"
+          "reifies_s s' i h' st' fs"
+          "reifies_loc locs' st'"
+          "snd (snd st') = lvar_st"
+  shows "res_wf lvar_st (fs,lesss,ress) (RValue rvs) locs' s' hf vcsf (St' \<^sub>s|\<^sub>h H')"
+  using assms
+proof -
+  have "\<exists>p pa vs pb. ass_sat (St' \<^sub>s|\<^sub>h H') vs pa pb \<and> vcsf @ vcs' = vcsf @ vs \<and> heap_disj pa hf \<and> p = heap_merge pa hf \<and> reifies_s s' i p pb fs \<and> reifies_loc locs' pb \<and> snd (snd pb) = lvar_st"
+    using assms by blast
+  then show ?thesis
+    by (simp add: assms(2) res_wf_def)
+qed
+
+lemma res_wf_intro_break:
+  assumes "k < length lesss"
+          "ass_sat (lesss ! k) vcs' h'' st'"
+          "rvs = vcs'"
+          "heap_disj h'' hf"
+          "h' = heap_merge h'' hf"
+          "reifies_s s' i h' st' fs"
+          "reifies_loc locs' st'"
+          "snd (snd st') = lvar_st"
+  shows "res_wf lvar_st (fs,lesss,ress) (RBreak k rvs) locs' s' hf vcsf (St' \<^sub>s|\<^sub>h H')"
+  using assms
+proof -
+
+  have "\<exists>h' h'' vcs' st'.
+              k < length lesss \<and>
+              ass_sat (lesss ! k) vcs' h''
+               st' \<and>
+              rvs = vcs' \<and>
+              heap_disj h'' hf \<and>
+              h' = heap_merge h'' hf \<and>
+              reifies_s s' i h' st' fs \<and>
+              reifies_loc locs' st' \<and>
+              snd (snd st') = lvar_st"
+    using assms
+    by blast
+  thus ?thesis
+    by (simp add: assms(2) res_wf_def)
+qed
+
+lemma res_wf_intro_return:
+  assumes "ress = Some the_ress"
+          "ass_sat the_ress vcs' h'' st'"
+          "rvs = vcs'"
+          "heap_disj h'' hf"
+          "h' = heap_merge h'' hf"
+          "reifies_s s' i h' st' fs"
+          "reifies_loc locs' st'"
+          "snd (snd st') = lvar_st"
+  shows "res_wf lvar_st (fs,lesss,ress) (RReturn rvs) locs' s' hf vcsf (St' \<^sub>s|\<^sub>h H')"
+  using assms
+proof -
+  have "\<exists>h' h'' vcs' st' the_rass.
+              ress = Some the_rass \<and>
+              ass_sat the_rass vcs' h'' st' \<and>
+              rvs = vcs' \<and>
+              heap_disj h'' hf \<and>
+              h' = heap_merge h'' hf \<and>
+              reifies_s s' i h' st' fs \<and>
+              reifies_loc locs' st' \<and>
+              snd (snd st') = lvar_st"
+    using assms
+    by blast
+  thus ?thesis
+    by (simp add: assms(2) res_wf_def)
+qed
+
+lemma stack_ass_sat_differ:
+  assumes "stack_ass_sat Stf vcs st"
+          "var_st_differ_on st vars st'"
+          "stack_ass_ind_on Stf vars"
+  shows "stack_ass_sat Stf vcs st'"
+  using assms
+  unfolding var_st_differ_on_def stack_ass_ind_on_def
+  by blast
+
+lemma heap_ass_sat_differ:
+  assumes "Hf h st"
+          "var_st_differ_on st vars st'"
+          "heap_ass_ind_on Hf vars"
+  shows "Hf h st'"
+  using assms
+  unfolding var_st_differ_on_def heap_ass_ind_on_def
+  by blast
+
+lemma res_wf_ext:
+  assumes "(ass_wf lvar_st ret \<Gamma> labs locs s hf st h (vcs_sf @ vcs_s) (Stf @ St \<^sub>s|\<^sub>h H))"
+          "(s,locs,($$*vcsf)@($$*vcs)@es) \<Down>n{(labs,ret,i)} (s',locs', (RValue res))"
+          "res_wf lvar_st \<Gamma> (RValue res) locs' s' hf (vcsf@vcs_sf) (St' \<^sub>s|\<^sub>h H')"
+          "stack_ass_ind_on Stf (modset (fst \<Gamma>) (($$*vcsf)@($$*vcs)@es))"
+          "stack_ass_sat Stf vcs_sf st"
+          "stack_ass_sat St vcs_s st"
+  shows "res_wf lvar_st \<Gamma> (RValue res) locs' s' hf vcsf (Stf @ St' \<^sub>s|\<^sub>h H')"
+proof -
+  have st_is:"ass_sat (Stf @ St \<^sub>s|\<^sub>h H) (vcs_sf @ vcs_s) h st"
+       "reifies_func (funcs s) (inst.funcs i) (fst \<Gamma>)"
+       "reifies_glob (globs s) (inst.globs i) st"
+       "reifies_loc locs st"
+       "snd (snd st) = lvar_st"
+    using assms(1)
+    unfolding ass_wf_def reifies_s_def
+    by auto
+  obtain  h' h'' vcs' st' where st'_is:
+          "ass_sat (St' \<^sub>s|\<^sub>h H') vcs' h''  st'"
+          "res = vcsf @ (vcs_sf @ vcs')"
+          "heap_disj h'' hf"
+          "h' = heap_merge h'' hf"
+          "reifies_s s' i h' st' (fst \<Gamma>)"
+          "reifies_loc locs' st'"
+          "snd (snd st') = lvar_st"
+    using assms(3)
+    unfolding res_wf_def
+    by fastforce
+  have 1:"reifies_glob (s.globs s') (inst.globs i) st'"
+    using st'_is(5)
+    unfolding reifies_s_def
+    by blast
+  have "ass_sat (Stf @ St' \<^sub>s|\<^sub>h H') (vcs_sf @ vcs') h'' st'"
+    using st'_is(1)
+          stack_ass_sat_differ[OF assms(5) _ assms(4)]
+          modifies_var_st[OF assms(2) st_is(2,3,4,5) 1 st'_is(6,7)]
+    by (simp add: list_all2_appendI stack_ass_sat_def)
+  thus ?thesis
+    using res_wf_intro_value[OF _ st'_is(2,3,4,5,6,7)]
+    by (metis prod.exhaust_sel)
+qed
+
+lemma res_wf_frame:
+  assumes "\<Gamma> = (fs, map (ass_frame Hf) ls, map_option (ass_frame Hf) rs)"
+          "(ass_wf lvar_st ret \<Gamma> labs locs s hf st (heap_merge h_H h_Hf) vcs (St \<^sub>s|\<^sub>h (H \<^emph> Hf)))"
+          "(s,locs,($$*vcsf)@($$*vcs)@es) \<Down>n{(labs,ret,i)} (s',locs', res)"
+          "res_wf lvar_st (fs,ls,rs) res locs' s' (heap_merge h_Hf hf) vcsf (St' \<^sub>s|\<^sub>h H')"
+          "heap_disj h_H h_Hf"
+          "H h_H st"
+          "Hf h_Hf st"
+          "heap_ass_ind_on Hf (modset fs es)"
+          "\<forall>ass\<in>set ls. \<exists>Sa Ha. ass = Sa \<^sub>s|\<^sub>h Ha"
+          "pred_option (\<lambda>ass. \<exists>Sa Ha. ass = Sa \<^sub>s|\<^sub>h Ha) rs"
+  shows "res_wf lvar_st \<Gamma> res locs' s' hf vcsf (St' \<^sub>s|\<^sub>h (H' \<^emph> Hf))"
+proof -
+  have st_is:"ass_sat (St \<^sub>s|\<^sub>h (H \<^emph> Hf)) vcs (heap_merge h_H h_Hf) st"
+       "reifies_func (funcs s) (inst.funcs i) (fst \<Gamma>)"
+       "reifies_glob (globs s) (inst.globs i) st"
+       "reifies_loc locs st"
+       "snd (snd st) = lvar_st"
+       "heap_disj (heap_merge h_H h_Hf) hf"
+       "reifies_heap (s.mem s) (inst.mem i) (heap_merge (heap_merge h_H h_Hf) hf)"
+    using assms(2)
+    unfolding ass_wf_def reifies_s_def
+    by auto
+  show ?thesis
+  proof (cases res)
+    case (RValue x1)
+    then obtain  h' h'' vcs' st' where st'_is:
+          "ass_sat (St' \<^sub>s|\<^sub>h H') vcs' h'' st'"
+          "x1 = vcsf @ vcs'"
+          "heap_disj h'' (heap_merge h_Hf hf)"
+          "h' = heap_merge h'' (heap_merge h_Hf hf)"
+          "reifies_s s' i h' st' fs"
+          "reifies_loc locs' st'"
+          "snd (snd st') = lvar_st"
+      using assms(4)
+      unfolding res_wf_def
+      by fastforce
+    have 0:"heap_disj h'' h_Hf"
+      using st'_is(3)
+      unfolding heap_disj_def heap_merge_def map_disj_def disjnt_def option_disj_def
+      by (auto split: option.splits prod.splits)
+    have 2:"H' h'' st'"
+      using st'_is(1)
+      by auto
+    have 1:"reifies_glob (s.globs s') (inst.globs i) st'"
+      using st'_is(5)
+      unfolding reifies_s_def
+      by blast
+    have 3:"Hf h_Hf st'"
+      using heap_ass_sat_differ[OF assms(7) _ assms(8)] assms(1) modset_consts_app[of _ fs "vcsf@vcs" es]
+            modifies_var_st[OF assms(3) st_is(2,3,4,5) 1 st'_is(6,7)]
+      by (simp add: var_st_differ_on_def)
+    have 4:"ass_sat (St' \<^sub>s|\<^sub>h (H' \<^emph> Hf)) vcs' (heap_merge h'' h_Hf) st'"
+      using st'_is(1) 3 0 2
+      apply ( simp add: list_all2_appendI sep_conj_def)
+      apply (metis prod.collapse)
+      done
+    have "heap_disj (heap_merge h'' h_Hf) hf"
+      by (metis heap_disj_merge_assoc heap_disj_merge_sub(2) heap_disj_sym st'_is(3) st_is(6))
+    thus ?thesis
+      using RValue res_wf_intro_value[OF 4 st'_is(2) _ _ st'_is(5,6,7)] assms(1) heap_merge_assoc st'_is(4)
+      by blast
+  next
+    case (RBreak x21 x22)
+    then obtain  h' h'' vcs' st' where st'_is:
+          "x21 < length ls"
+          "ass_sat (ls ! x21) vcs' h'' st'"
+          "x22 = vcs'"
+          "heap_disj h'' (heap_merge h_Hf hf)"
+          "h' = heap_merge h'' (heap_merge h_Hf hf)"
+          "reifies_s s' i h' st' fs"
+          "reifies_loc locs' st'"
+          "snd (snd st') = lvar_st"
+      using assms(4)
+      unfolding res_wf_def
+      by fastforce
+    have 0:"heap_disj h'' h_Hf"
+      using st'_is(4)
+      unfolding heap_disj_def heap_merge_def map_disj_def disjnt_def option_disj_def
+      by (auto split: option.splits prod.splits)
+    obtain Hr Str where lsi:"(ls ! x21) = Str \<^sub>s|\<^sub>h Hr"
+      using assms(9) st'_is(1) nth_mem
+      by blast
+    have 2:"Hr h'' st'"
+      using st'_is(2) lsi
+      by auto
+    have 1:"reifies_glob (s.globs s') (inst.globs i) st'"
+      using st'_is(6)
+      unfolding reifies_s_def
+      by blast
+    have 3:"Hf h_Hf st'"
+      using heap_ass_sat_differ[OF assms(7) _ assms(8)] assms(1) modset_consts_app[of _ fs "vcsf@vcs" es]
+            modifies_var_st[OF assms(3) st_is(2,3,4,5) 1 st'_is(7,8)]
+      by (simp add: var_st_differ_on_def)
+    have 4:"ass_sat (Str \<^sub>s|\<^sub>h (Hr \<^emph> Hf)) vcs' (heap_merge h'' h_Hf) st'"
+      using st'_is(2) 3 0 2 lsi
+      apply (simp add: list_all2_appendI sep_conj_def)
+      apply (metis prod.collapse)
+      done
+    have 5:"heap_disj (heap_merge h'' h_Hf) hf"
+      by (metis heap_disj_merge_assoc heap_disj_merge_sub(2) heap_disj_sym st'_is(4) st_is(6))
+    have 6:"(map (ass_frame Hf) ls)!x21 = (Str \<^sub>s|\<^sub>h (Hr \<^emph> Hf))"
+      using st'_is(1) lsi
+      unfolding ass_frame_def
+      by auto
+    show ?thesis
+      using RBreak res_wf_intro_break[OF _ _ _ 5 _ st'_is(6,7,8)] assms(1) heap_merge_assoc 4 6 st'_is(1,3,5)
+      by auto
+  next
+    case RTrap
+    thus ?thesis
+      using assms(4)
+      unfolding res_wf_def
+      by auto
+  next
+    case (RReturn x3)
+    then obtain  h' h'' vcs' st' the_rass where st'_is:
+          "rs = Some the_rass"
+          "ass_sat the_rass vcs' h'' st'"
+          "x3 = vcs'"
+          "heap_disj h'' (heap_merge h_Hf hf)"
+          "h' = heap_merge h'' (heap_merge h_Hf hf)"
+          "reifies_s s' i h' st' fs"
+          "reifies_loc locs' st'"
+          "snd (snd st') = lvar_st"
+      using assms(4)
+      unfolding res_wf_def
+      by fastforce
+    have 0:"heap_disj h'' h_Hf"
+      using st'_is(4)
+      unfolding heap_disj_def heap_merge_def map_disj_def disjnt_def option_disj_def
+      by (auto split: option.splits prod.splits)
+    obtain Hr Str where rass_def:"the_rass = Str \<^sub>s|\<^sub>h Hr"
+      using assms(10) st'_is(1)
+      by auto
+    have 2:"Hr h'' st'"
+      using st'_is(2) rass_def
+      by auto
+    have 1:"reifies_glob (s.globs s') (inst.globs i) st'"
+      using st'_is(6)
+      unfolding reifies_s_def
+      by blast
+    have 3:"Hf h_Hf st'"
+      using heap_ass_sat_differ[OF assms(7) _ assms(8)] assms(1) modset_consts_app[of _ fs "vcsf@vcs" es]
+            modifies_var_st[OF assms(3) st_is(2,3,4,5) 1 st'_is(7,8)]
+      by (simp add: var_st_differ_on_def)
+    have 4:"ass_sat (Str \<^sub>s|\<^sub>h (Hr \<^emph> Hf)) vcs' (heap_merge h'' h_Hf) st'"
+      using st'_is(2) 3 0 2 rass_def
+      apply (simp add: list_all2_appendI sep_conj_def)
+      apply (metis prod.collapse)
+      done
+    have 5:"heap_disj (heap_merge h'' h_Hf) hf"
+      by (metis heap_disj_merge_assoc heap_disj_merge_sub(2) heap_disj_sym st'_is(4) st_is(6))
+    have 6:"map_option (ass_frame Hf) rs = Some (Str \<^sub>s|\<^sub>h (Hr \<^emph> Hf))"
+      using st'_is(1) rass_def
+      unfolding ass_frame_def
+      by auto
+    show ?thesis
+      using RReturn res_wf_intro_return[OF 6 4 st'_is(3) 5 _ st'_is(6,7,8)] assms(1) heap_merge_assoc st'_is(5)
+      by blast
+  qed
 qed
 
 lemma valid_triples_n_call_equiv_callcl:
@@ -287,8 +723,20 @@ next
   then show ?case sorry
 next
   case (Asm P k Q assms \<Gamma>)
+  {
+    assume "((fst \<Gamma>,[],None) \<TTurnstile>_n assms)"
+    hence "((fst \<Gamma>,[],None) \<TTurnstile>_n {(P, [$Call k], Q)})"
+      using Asm
+      by (metis singletonD valid_triples_n_def)
+    hence "\<Gamma> \<TTurnstile>_ n {(P, [$Call k], Q)}"
+      using extend_context_call
+      apply (cases \<Gamma>)
+      apply (simp add: valid_triple_defs(5) extend_context_call)
+      done
+  }
   thus ?case
-    by (metis valid_triple_defs(5) valid_triples_assms_n_def singletonD)
+    unfolding valid_triples_assms_n_def
+    by blast
 next
   case (Seq \<Gamma> assms P es Q es' R)
   then show ?case sorry
@@ -298,13 +746,88 @@ next
     using valid_triple_assms_n_conseq
     by blast
 next
-  case (Frame \<Gamma> assms St H es St' H' Hf)
+  case (Frame fs ls rs assms St H es St' H' Hf)
+  {
+    fix vcs h st s locs labs ret lvar_st vcsf s' locs' res hf \<Gamma>
+    assume local_assms:"\<Gamma> = (fs, map (ass_frame Hf) ls,  map_option (ass_frame Hf) rs)"
+                       "(fst \<Gamma>,[],None) \<TTurnstile>_n assms"
+                       "(ass_wf lvar_st ret \<Gamma> labs locs s hf st h vcs (St \<^sub>s|\<^sub>h (H \<^emph> Hf)))"
+                       "(s,locs,($$*vcsf)@($$*vcs)@es) \<Down>n{(labs,ret,i)} (s',locs', res)"
+    then obtain h_H h_Hf where h_H_def:"heap_disj h_H h_Hf"
+                                       "H h_H st"
+                                       "Hf h_Hf st"
+                                       "heap_merge h_H h_Hf = h"
+      unfolding ass_wf_def sep_conj_def
+      by fastforce
+    hence 0:"(ass_wf lvar_st ret \<Gamma> labs locs s (heap_merge h_Hf hf) st h_H vcs (St \<^sub>s|\<^sub>h H))"
+      using sep_conj_imp_frame local_assms(1,3) heap_disj_merge_assoc heap_merge_assoc
+      unfolding ass_wf_def sep_conj_def
+      by auto
+    hence 1:"(ass_wf lvar_st ret (fs, ls, rs) labs locs s (heap_merge h_Hf hf) st h_H vcs (St \<^sub>s|\<^sub>h H))"
+      using reifies_lab_ass_frame_inv reifies_ret_ass_frame_inv local_assms(1)
+      unfolding ass_wf_def
+      by (metis fstI prod.sel(2) reifies_lab_def reifies_ret_def)
+    have "((fs, ls, rs) \<Turnstile>_n {(St \<^sub>s|\<^sub>h H)}es{(St' \<^sub>s|\<^sub>h H')})"
+      using local_assms(1,2) Frame(5)
+      unfolding valid_triples_assms_n_def valid_triples_n_def
+      by auto
+    hence "res_wf lvar_st (fs, ls, rs) res locs' s' (heap_merge h_Hf hf) vcsf (St' \<^sub>s|\<^sub>h H')"
+      using local_assms(4) 1
+      unfolding valid_triple_defs
+      by metis
+    hence "res_wf lvar_st \<Gamma> res locs' s' hf vcsf (St' \<^sub>s|\<^sub>h (H' \<^emph> Hf))"
+      using res_wf_frame[OF local_assms(1) _ local_assms(4) _ h_H_def(1) _ _ _ Frame(3,4)]
+            Frame(2) h_H_def(2,3,4) local_assms(3)
+      by blast
+  }
   thus ?case
-    sorry
+    unfolding valid_triple_defs
+    by auto
 next
   case (Ext \<Gamma> assms St H es St' H' Stf)
+  {
+    fix vcs h st s locs labs ret lvar_st vcsf s' locs' res hf
+    assume local_assms:"(fst \<Gamma>,[],None) \<TTurnstile>_n assms"
+                       "(ass_wf lvar_st ret \<Gamma> labs locs s hf st h vcs (Stf @ St \<^sub>s|\<^sub>h H))"
+                       "(s,locs,($$*vcsf)@($$*vcs)@es) \<Down>n{(labs,ret,i)} (s',locs', res)"
+    obtain vcs' vcs'' where vcs_is:"stack_ass_sat (Stf @ St) vcs st"
+                                    "stack_ass_sat Stf vcs' st"
+                                    "stack_ass_sat St vcs'' st"
+                                    "vcs = vcs'@vcs''"
+      using local_assms(2)
+      unfolding ass_wf_def
+      by (fastforce simp add: stack_ass_sat_def list_all2_append1)
+    hence 1:"(ass_wf lvar_st ret \<Gamma> labs locs s hf st h vcs'' (St \<^sub>s|\<^sub>h H))"
+      using local_assms(2)
+      unfolding ass_wf_def ass_sat.simps
+      by simp
+    have "(\<Gamma> \<Turnstile>_n {(St \<^sub>s|\<^sub>h H)}es{(St' \<^sub>s|\<^sub>h H')})"
+      using local_assms(1) Ext(3)[of n]
+      unfolding valid_triples_assms_n_def valid_triples_n_def
+      by auto
+    hence 2:"res_wf lvar_st \<Gamma> res locs' s' hf (vcsf@vcs') (St' \<^sub>s|\<^sub>h H')"
+      using local_assms(3) 1
+      unfolding valid_triple_defs
+      by (metis vcs_is(4) append.assoc map_append)
+    hence "res_wf lvar_st \<Gamma> res locs' s' hf vcsf (Stf @ St' \<^sub>s|\<^sub>h H')"
+    proof (cases res)
+      case (RValue x1)
+      hence 3:"(ass_wf lvar_st ret \<Gamma> labs locs s hf st h (vcs'@vcs'') (Stf @ St \<^sub>s|\<^sub>h H))"
+              "(s,locs,($$*vcsf)@($$*vcs)@es) \<Down>n{(labs,ret,i)} (s',locs', (RValue x1))"
+              "res_wf lvar_st \<Gamma> (RValue x1) locs' s' hf (vcsf@vcs') (St' \<^sub>s|\<^sub>h H')"
+        using local_assms(2,3) vcs_is(4) 2
+        by auto
+      have "stack_ass_ind_on Stf (modset (fst \<Gamma>) (($$* vcsf) @ ($$* vcs) @ es))"
+        using Ext(2) modset_consts_app
+        by (metis Collect_cong modifies_modset_eq modset_def)
+      thus ?thesis
+        using res_wf_ext[OF 3(1,2,3) _ vcs_is(2,3)] RValue
+        by fastforce
+    qed (auto simp add: res_wf_def)
+  }
   thus ?case
-    sorry
+    unfolding valid_triple_defs
+    by auto
 next
   case (Call fs specs)
   show ?case
@@ -333,9 +856,9 @@ next
       using Suc(1)[OF Suc(2,3)]
       by -
     hence "(fs, [], None) \<TTurnstile>_ n {(P, c, Q). \<exists>i. (P, [$Call i], Q) \<in> specs \<and> i < length fs \<and> c = [Callcl (fs ! i)]}"
-      using Suc(3)[of n] valid_triples_n_emp
+      using Suc(3)[of n]
       unfolding valid_triples_assms_n_def
-      by blast
+      by (simp add: valid_triples_n_emp)
     thus ?case
       using valid_triples_n_call_equiv_callcl[OF _ Suc(2)]
       by blast
